Finish the formal verification effort (#56)
---------

Co-authored-by: Giuseppe <8973725+Eagle941@users.noreply.github.com>

formal-verification/Main.lean
@@ -1,140 +1,360 @@
-import ProvenZk.Binary
-import ProvenZk.Hash
-import ProvenZk.Merkle
-import ProvenZk.Ext.Vector
-
+import ProvenZk
 import FormalVerification
-import FormalVerification.Poseidon.Spec
-import FormalVerification.Poseidon.Correctness
-import FormalVerification.SemanticEquivalence
+import FormalVerification.Insertion
+import FormalVerification.Deletion
+import FormalVerification.Common
+import FormalVerification.Poseidon
+import FormalVerification.InputHashing
+import FormalVerification.ReducednessCheck
+import FormalVerification.BinaryDecompositions
 
 open SemaphoreMTB (F Order)
 
-variable [Fact (Nat.Prime Order)]
 
-open SemaphoreMTB renaming VerifyProof_31_30 → gVerifyProof
-open SemaphoreMTB renaming DeletionRound_30_30 → gDeletionRound
-open SemaphoreMTB renaming DeletionProof_4_4_30_4_4_30 → gDeletionProof
-open SemaphoreMTB renaming InsertionRound_30_30 → gInsertionRound
-open SemaphoreMTB renaming InsertionProof_4_30_4_4_30 → gInsertionProof
+namespace Poseidon
 
-def TreeInsert [Fact (perfect_hash poseidon₂)] (Tree : MerkleTree F poseidon₂ D) (Index Item : F) (Proof : Vector F D) (k : F → Prop): Prop :=
-  MerkleTree.item_at_nat Tree Index.val = some 0 ∧
-  MerkleTree.proof_at_nat Tree Index.val = some Proof.reverse ∧
-  ∃postTree, MerkleTree.set_at_nat Tree Index.val Item = some postTree ∧
-  k postTree.root
+/--
+Tests the Poseidon implementation automatically derived from the circuit, by
+comparing its output on an arbitrary value to a reference value.
 
-theorem insertion_round_uncps [Fact (perfect_hash poseidon₂)] (Tree : MerkleTree F poseidon₂ D) (Index Item : F) (Proof : Vector F D) (k : F → Prop):
-  insertion_round Index Item Tree.root Proof k ↔
-  TreeInsert Tree Index Item Proof k := by
-  unfold insertion_round
-  unfold TreeInsert
-  apply Iff.intro
-  . rintro ⟨ixbin, _⟩
-    casesm* (_ ∧ _)
-    have : nat_to_bits_le D Index.val = some (vector_zmod_to_bit ixbin) := by
-      apply recover_binary_zmod'_to_bits_le
-      . simp
-      . assumption
-      . rename_i h _ _ _; simp[h]
-    unfold MerkleTree.item_at_nat
-    unfold MerkleTree.proof_at_nat
-    unfold MerkleTree.set_at_nat
-    unfold Dir.nat_to_dir_vec
-    rw [this]
-    simp [←Dir.create_dir_vec_bit]
-    rename_i h₀ h₁ h₂ h₃
-    refine ⟨?_, ⟨?_, ?_⟩⟩
-    . apply MerkleTree.proof_ceritfies_item (proof := Proof.reverse)
-      rw [←MerkleTree.recover_tail_reverse_equals_recover]
-      simp [h₂]
-    . apply MerkleTree.recover_proof_reversible
-      rw [←MerkleTree.recover_tail_reverse_equals_recover (item := (0:F))]
-      simp [h₂]
-    . rw [←MerkleTree.proof_insert_invariant (proof := Proof.reverse) (old := 0)]
-      . rw [←MerkleTree.recover_tail_reverse_equals_recover]
-        simp [h₃]
-      . rw [←MerkleTree.recover_tail_reverse_equals_recover]
-        simp [h₂]
-  . rintro ⟨hitem, ⟨hproof, ⟨ftree, ⟨hftree, hresult⟩⟩⟩⟩
-    simp [MerkleTree.item_at_nat, Dir.nat_to_dir_vec] at hitem
-    rcases hitem with ⟨bits, ⟨hbits, hitem_at⟩⟩
-    simp [MerkleTree.proof_at_nat, Dir.nat_to_dir_vec] at hproof
-    rcases hproof with ⟨bits', ⟨hbits', hproof_at⟩⟩
-    simp [hbits] at hbits'
-    simp [hbits'] at *
-    simp [MerkleTree.set_at_nat, Dir.nat_to_dir_vec] at hftree
-    rcases hftree with ⟨bits'', ⟨hbits'', hftree_at⟩⟩
-    simp [hbits''] at hbits
-    rw [←Vector.vector_reverse_eq] at hproof_at
-    simp [hbits] at *
-    simp [<-hproof_at]
-    let t : Vector F D := (Vector.map Bit.toZMod bits')
-    refine ⟨t, ?_⟩
-    refine ⟨?_, ⟨?_, ⟨?_, ?_⟩⟩⟩
-    . apply recover_binary_of_to_bits
-      simp [hbits'']
-    . apply vector_binary_of_bit_to_zmod
-    . rw [MerkleTree.recover_tail_equals_recover_reverse, Dir.create_dir_vec_bit, zmod_to_bit_coe, ←hitem_at]
-      simp [MerkleTree.recover_proof_is_root]
-    . rw [<-hftree_at] at hresult
-      rw [MerkleTree.recover_tail_equals_recover_reverse, Dir.create_dir_vec_bit, zmod_to_bit_coe]
-      rw [MerkleTree.proof_insert_invariant _]
-      . apply hresult
-      . exact 0
-      . rw [← hitem_at]
-        simp [MerkleTree.recover_proof_is_root]
+The reference value is taken from
+<https://extgit.iaik.tugraz.at/krypto/hadeshash/blob/master/code/test_vectors.txt>
+-/
+theorem poseidon₂_test:
+    poseidon₂ vec![1,2] = 0x115cc0f5e7d690413df64c6b9662e9cf2a3617f2743245519e19607a4417189a
+  := by native_decide
 
-theorem before_insertion_all_items_zero_loop
-  [Fact (perfect_hash poseidon₂)]
-  {Tree: MerkleTree F poseidon₂ D}
-  {StartIndex B: Nat}
-  {ixBound: StartIndex + B < Order}
-  {IdComms: Vector F B} {MerkleProofs: Vector (Vector F D) B} {k: F -> Prop}:
-  insertion_rounds ↑StartIndex Tree.root IdComms MerkleProofs k →
-  (∀ i ∈ [StartIndex:StartIndex + B], MerkleTree.item_at_nat Tree i = some 0) := by
-  induction B generalizing StartIndex Tree with
-  | zero =>
-    intro _ i range
-    rcases range with ⟨lo, hi⟩
-    have := Nat.ne_of_lt (Nat.lt_of_le_of_lt lo hi)
-    contradiction
-  | succ B ih =>
-    intro hp i range
-    rcases range with ⟨lo, hi⟩; simp at lo hi
-    have hStartIndexCast : ZMod.val (StartIndex : F) = StartIndex := by
-      apply ZMod.val_cast_of_lt
-      linarith
-    cases lo with
-    | refl =>
-      simp [insertion_rounds,  InsertionRound_uncps, insertion_round_uncps, TreeInsert, hStartIndexCast] at hp
-      cases hp
-      rename_i l r
-      simp [l]
-    | @step StartIndex' h =>
-      have : (StartIndex : F) + 1 = ((StartIndex + 1 : Nat) : F) := by
-        simp [Fin.ext]
-      rw [insertion_rounds,  InsertionRound_uncps, insertion_round_uncps, TreeInsert, this] at hp
-      rcases hp with ⟨_, ⟨_, ⟨postTree, ⟨hinsert, hnext⟩⟩⟩⟩
-      rw [←MerkleTree.item_at_nat_invariant hinsert]
-      apply ih hnext StartIndex'.succ
-      . apply And.intro
-        . simp_arith; simp [Nat.le] at h; simp [h]
-        . simp; linarith
-      . linarith
-      . rw [hStartIndexCast]
-        apply Nat.ne_of_lt
-        simp_arith; simp [Nat.le] at h; simp [h]
+end Poseidon
 
+namespace Deletion
+
+/--
+States the exact semantics of the deletion circuit.
+Whenever the circuit is satisfied, there exists a Merkle tree, such that:
+1. its root is equal to the one given as the `postRoot` input;
+2. for every index `i` in `deletionIndices`, the value at index `i` is zero;
+3. for every index `i` not in `deletionIndices`, the value at index `i` is
+   unchanged.
+-/
+theorem root_transformation_correct
+  [Fact (CollisionResistant poseidon₂)]
+  {tree : MerkleTree F poseidon₂ D}:
+    SemaphoreMTB.DeletionMbuCircuit_4_4_30_4_4_30 inputHash deletionIndices tree.root postRoot identities merkleProofs →
+    ∃(postTree : MerkleTree F poseidon₂ D),
+    postTree.root = postRoot ∧
+    (∀ i ∈ deletionIndices, postTree[i.val]! = 0) ∧
+    (∀ i, i ∉ deletionIndices → postTree[i.val]! = tree[i.val]!)
+  := by
+  intro hp
+  replace hp := Deletion_skipHashing hp
+  rw [deletionProofCircuit_eq_deletionRoundsSemantics] at hp
+  replace hp := deletionRounds_rootTransformation hp
+  rcases hp with ⟨postTree, treeTrans, rootTrans⟩
+  exists postTree
+  refine ⟨rootTrans, ?inrange, ?outrange⟩
+  . intro i hi
+    apply treeTranform_get_present treeTrans hi
+  . intro i hi
+    simp [getElem!_eq_getElem?_get!]
+    apply congrArg
+    apply treeTransform_get_absent treeTrans hi
+
+/--
+States that for any given tree and list of valid indices, there exists a choice
+of other parameters, such that the deletion circuit is satisfied. As a corollary,
+we can be certain that the system will always be able to remove any identity from
+the tree.
+NB indices are consider valid if they are less than 2ᴰ⁺¹, where D is the merkle
+tree depth. This allows the circuit to use indices larger than the tree size to
+pad batches.
+-/
+theorem assignment_exists
+  [Fact (CollisionResistant poseidon₂)]
+  {tree : MerkleTree F poseidon₂ D}
+  {indices : Vector F B}:
+    (∀i ∈ indices, i.val < 2^(D+1)) →
+    ∃inputHash identities proofs postRoot, SemaphoreMTB.DeletionMbuCircuit_4_4_30_4_4_30 inputHash indices tree.root postRoot identities proofs
+  := by
+  intro h;
+  simp only [DeletionCircuit_folded, DeletionMbuCircuit_4_4_30_4_4_30_Fold]
+  simp only [
+    Vector.ofFnGet_id,
+    ToReducedBigEndian_32_uncps,
+    ToReducedBigEndian_256_uncps,
+    RCBitsField_def,
+    ←Vector.map_permute,
+    Vector.map_hAppend,
+    (KeccakGadget_640_64_24_640_256_24_1088_1_uniqueAssignment _ _).equiv,
+    FromBinaryBigEndian_256_uncps,
+    Gates.eq,
+    deletionProofCircuit_eq_deletionRoundsSemantics
+  ]
+  have := exists_assignment (tree := tree) h
+  rcases this with ⟨_, _, _, hp⟩
+  repeat apply Exists.intro
+  apply And.intro (Eq.refl _)
+  simp
+  apply hp
+  simp only [D] at h
+  all_goals {
+    apply Nat.lt_trans _ ((by decide) : 2 ^ 31 < 2 ^ 32)
+    apply h
+    simp [getElem]
+  }
+
+/--
+Establishes that the deletion circuit's InputHash parameter is uniquely
+determined by DeletionIndices, PreRoot and PostRoot. That is done by showing
+that any two valid assigments that agree on those parameters, must also agree
+on InputHash.
+-/
+theorem inputHash_deterministic:
+    (SemaphoreMTB.DeletionMbuCircuit_4_4_30_4_4_30 InputHash₁ DeletionIndices PreRoot PostRoot IdComms₁ MerkleProofs₁ ∧
+     SemaphoreMTB.DeletionMbuCircuit_4_4_30_4_4_30 InputHash₂ DeletionIndices PreRoot PostRoot IdComms₂ MerkleProofs₂)
+    → InputHash₁ = InputHash₂
+  := Deletion_InputHash_deterministic
+
+/--
+Arbitrary string used for testing the 640-bit keccak hash implementation.
+-/
+def testString80 : String :=
+  "This string is exactly 80 bytes long, which is unbelievably lucky for this test."
+
+/--
+An embedding of the test string into a vector of bits, by taking the little-endian
+bit decomposition of the ASCII value of each character.
+-/
+def testVector640 : Vector Bool 640 :=
+  Subtype.mk (testString80.toUTF8.toList.map (fun b => Vector.toList $ Fin.toBitsLE (d := 8) b.val)).join (by native_decide)
+
+/--
+Tests the Keccak implementation automatically derived from the circuit, by
+comparing its output on an arbitrary value to a reference value computed using
+solidity.
+
+The reference number is obtained by hashing the test string using the following Solidity code:
+```solidity
+string memory data = "This string is exactly 80 bytes long, which is unbelievably lucky for this test.";
+uint256 result;
+assembly {
+  result := mod(keccak256(add(data, 0x20), mload(data)), 0x30644e72e131a029b85045b68181585d2833e84879b9709143e1f593f0000001)
+}
+```
+-/
+theorem reducedKeccak640_test :
+  reducedKeccak640 testVector640 = 0x799e635101207dc20689c342be25dc6f5a2f25b51d2a5ac3c9fee51694b3609 := by native_decide
+
+/--
+This axiom is necessary for the proof of the injectivity of the input hash
+parameter. It is obviously not true (e.g. by the pigeonhole principle), but it
+captures the usual intuition behind hash functions.
+-/
+axiom reducedKeccak640_collision_resistant :
+  ∀x y, reducedKeccak640 x = reducedKeccak640 y → x = y
+
+/--
+States that the input hash parameter is injective. That is, if two valid
+assignments share the same input hash, then they must agree on all other public
+parameters.
+-/
+theorem inputHash_injective:
+    SemaphoreMTB.DeletionMbuCircuit_4_4_30_4_4_30 InputHash DeletionIndices₁ PreRoot₁ PostRoot₁ IdComms₁ MerkleProofs₁ ∧
+    SemaphoreMTB.DeletionMbuCircuit_4_4_30_4_4_30 InputHash DeletionIndices₂ PreRoot₂ PostRoot₂ IdComms₂ MerkleProofs₂ →
+    DeletionIndices₁ = DeletionIndices₂ ∧ PreRoot₁ = PreRoot₂ ∧ PostRoot₁ = PostRoot₂
+  := Deletion_InputHash_injective reducedKeccak640_collision_resistant
+
+end Deletion
+
+namespace Insertion
+
+/--
+Checks input validation on the insertion circuit. The circuit being satisfied
+implies that all items at modified indices are zero, therefore it is impossible
+to use this circuit to, either accidentally or malicious, overwrite existing
+data.
+-/
 theorem before_insertion_all_items_zero
-  [Fact (perfect_hash poseidon₂)]
-  {Tree: MerkleTree F poseidon₂ D}
-  (StartIndex: Nat) (IdComms: Vector F B) (MerkleProofs: Vector (Vector F D) B) (k: F -> Prop)
-  {ixBound: StartIndex + B < Order}:
-  gInsertionProof ↑StartIndex Tree.root IdComms MerkleProofs k →
-  (∀ i ∈ [StartIndex:StartIndex + B], MerkleTree.item_at_nat Tree i = some 0) := by
-  rw [InsertionProof_looped]
-  apply before_insertion_all_items_zero_loop
-  simp [ixBound]
+  [Fact (CollisionResistant poseidon₂)]
+  {tree: MerkleTree F poseidon₂ D}
+  {startIndex : F}:
+    SemaphoreMTB.InsertionMbuCircuit_4_30_4_4_30 InputHash startIndex tree.root PostRoot IdComms MerkleProofs →
+    ∀ i ∈ [startIndex.val:startIndex.val + B], tree[i]! = 0
+  := by
+  intro hp i hir
+  have hp := Insertion_skipHashing hp
+  rw [Insertion.insertionRoundsCircuit_eq_insertionRoundsSemantics] at hp
+  have hp'' := ix_bound hp
+  rw [getElem!_eq_getElem?_get!]
+  rw [before_insertion_all_zero hp]; rfl
+  apply And.intro
+  . exact hir.1
+  . apply Nat.lt_of_lt_of_eq hir.2
+    rw [ZMod.val_add, Nat.mod_eq_of_lt]
+    rfl
+    calc
+      startIndex.val + 4 = (startIndex.val + 3) + 1 := by ring
+      _ < 2^D + 1 := Nat.add_lt_add_right hp'' (k := 1)
+      _ < Order := by decide
 
-def main : IO Unit := pure ()
+/--
+States the exact semantics of the insertion circuit.
+Whenever the circuit is satisfied, there exists a Merkle tree, such that:
+1. its root is equal to the one given as the `postRoot` input;
+2. for every index `i` such that `startIndex ≤ i < startIndex + B`, the value
+   at index `i` is equal to `idComms[i-startIndex]`;
+3. for every index `i` outside the specified range, the value at index `i`
+   remains unchanged.
+-/
+theorem root_transformation_correct
+    [Fact (CollisionResistant poseidon₂)]
+    {Tree : MerkleTree F poseidon₂ D}:
+    SemaphoreMTB.InsertionMbuCircuit_4_30_4_4_30 InputHash StartIndex Tree.root PostRoot IdComms MerkleProofs →
+    ∃(postTree : MerkleTree F poseidon₂ D),
+    postTree.root = PostRoot ∧
+    (∀ i, i ∈ [StartIndex.val:StartIndex.val + B] → postTree[i]! = IdComms[i-StartIndex.val]!) ∧
+    (∀ i, i ∉ [StartIndex.val:StartIndex.val + B] → postTree[i]! = Tree[i]!)
+  := by
+  intro hp
+  have hp := Insertion_skipHashing hp
+  rw [insertionRoundsCircuit_eq_insertionRoundsSemantics] at hp
+  have hp := insertionRoundsRootTransformation hp
+  rcases hp with ⟨postTree, treeTrans, rootTrans⟩
+  exists postTree
+  simp_rw [getElem!_eq_getElem?_get!]
+  refine ⟨rootTrans, ?inrange, ?outrange⟩
+  case inrange =>
+    intro i hi
+    have : i = StartIndex.val + (i - StartIndex.val) := by
+      rw [add_comm, Nat.sub_add_cancel hi.1]
+    have i_off_inrange : i - StartIndex.val ∈ [0:B] := by
+      refine ⟨Nat.zero_le _, ?_⟩
+      cases hi
+      linarith
+    rw [this, treeTransform_get_inrange treeTrans i_off_inrange, ←this]
+    apply congrArg
+    apply eq_comm.mp
+    apply getElem?_eq_some_getElem_of_valid_index
+  case outrange =>
+    intro i hi
+    cases Nat.lt_or_ge i StartIndex.val with
+    | inl h =>
+      apply congrArg
+      apply eq_comm.mp
+      apply treeTransform_get_lt treeTrans h
+    | inr h =>
+      cases Nat.lt_or_ge i (StartIndex.val + B) with
+      | inl h' =>
+        exfalso
+        exact hi ⟨h, h'⟩
+      | inr h =>
+        apply congrArg
+        apply eq_comm.mp
+        apply treeTransform_get_gt treeTrans h
+
+/--
+States that for any given tree, a valid start index, and a list of identities,
+there exists a choice of the other parameters such that the insertion circuit
+is satisfied. As a corollary, we can be certain that the system will always be
+able to progress, as long as there is enough free space in the tree.
+
+NB a start index is considered valid if it denotes the beginning of a length-B
+block of empty leaves.
+-/
+theorem assignment_exists [Fact (CollisionResistant poseidon₂)] {tree : MerkleTree F poseidon₂ D}:
+    startIndex + B < 2 ^ D ∧
+    (∀i ∈ [startIndex : startIndex + B], tree[i]! = 0) →
+    ∃proofs postRoot inputHash, SemaphoreMTB.InsertionMbuCircuit_4_30_4_4_30 inputHash startIndex tree.root postRoot idComms proofs
+  := by
+  rintro ⟨ix_ok, items_zero⟩
+  simp only [InsertionMbuCircuit_4_30_4_4_30_folded]
+  unfold InsertionMbuCircuit_4_30_4_4_30_Fold
+  simp only [
+    Vector.ofFnGet_id,
+    ToReducedBigEndian_32_uncps,
+    ToReducedBigEndian_256_uncps,
+    RCBitsField_def,
+    ←Vector.map_permute,
+    Vector.map_hAppend,
+    (KeccakGadget_1568_64_24_1568_256_24_1088_1_uniqueAssignment _ _).equiv,
+    FromBinaryBigEndian_256_uncps,
+    Gates.eq
+  ]
+  simp [insertionRoundsCircuit_eq_insertionRoundsSemantics]
+  have := exists_assignment (identities := idComms) ix_ok (by
+    intro i h
+    apply getElem_of_getElem!
+    apply items_zero
+    assumption
+  )
+  rcases this with ⟨proofs, postRoot, h⟩
+  exists proofs, postRoot
+  apply And.intro
+  . apply Exists.intro
+    apply Exists.intro
+    . rfl
+    . simp only [D, B] at ix_ok
+      rw [ZMod.val_cast_of_lt]
+      . linarith
+      . simp only [Order]; linarith
+  . exact h
+
+/--
+Establishes that the insertion circuit's InputHash parameter is uniquely
+determined by StartIndex, PreRoot, PostRoot and the identity commitments. That
+is done by showing that any two valid assigments that agree on those
+parameters, must also agree on InputHash.
+-/
+theorem inputHash_deterministic:
+    SemaphoreMTB.InsertionMbuCircuit_4_30_4_4_30 InputHash₁ StartIndex PreRoot PostRoot IdComms MerkleProofs₁ ∧
+    SemaphoreMTB.InsertionMbuCircuit_4_30_4_4_30 InputHash₂ StartIndex PreRoot PostRoot IdComms MerkleProofs₂ →
+    InputHash₁ = InputHash₂
+  := Insertion_InputHash_deterministic
+
+/--
+Arbitrary string used for testing the 1568-bit keccak hash implementation.
+-/
+def testString196 : String :=
+  "This is string is exactly 196 bytes long, which happens to be exactly the length we need to test the 1568-bit keccak hash implementation, that can be found in the SemaphoreMTB Insertion Circuit..."
+
+/--
+An embedding of the test string into a vector of bits, by taking the little-endian
+bit decomposition of the ASCII value of each character.
+-/
+def testVector1568 : Vector Bool 1568 :=
+  Subtype.mk (testString196.toUTF8.toList.map (fun b => Vector.toList $ Fin.toBitsLE (d := 8) b.val)).join (by native_decide)
+
+/--
+The reference number is obtained by hashing the test string using the following Solidity code:
+```solidity
+string memory data = "This is string is exactly 196 bytes long, which happens to be exactly the length we need to test the 1568-bit keccak hash implementation, that can be found in the SemaphoreMTB Insertion Circuit...";
+uint256 result;
+assembly {
+  result := mod(keccak256(add(data, 0x20), mload(data)), 0x30644e72e131a029b85045b68181585d2833e84879b9709143e1f593f0000001)
+}
+```
+-/
+theorem reducedKeccak1568_test :
+  reducedKeccak1568 testVector1568 = 0x204e42742e70b563e147bca3aac705534bfae2e7d17691127dd6425b23f5ba43 := by native_decide
+
+/--
+This axiom is necessary for the proof of the injectivity of the input hash
+parameter. It is obviously not true (e.g. by the pigeonhole principle), but it
+captures the usual intuition behind hash functions.
+-/
+axiom reducedKeccak1568_collision_resistant :
+  ∀x y, reducedKeccak1568 x = reducedKeccak1568 y → x = y
+
+/--
+States that the input hash parameter is injective. That is, if two valid
+assignments share the same input hash, then they must agree on all other public
+parameters.
+-/
+theorem inputHash_injective:
+  SemaphoreMTB.InsertionMbuCircuit_4_30_4_4_30 InputHash StartIndex₁ PreRoot₁ PostRoot₁ IdComms₁ MerkleProofs₁ ∧
+  SemaphoreMTB.InsertionMbuCircuit_4_30_4_4_30 InputHash StartIndex₂ PreRoot₂ PostRoot₂ IdComms₂ MerkleProofs₂ →
+  StartIndex₁ = StartIndex₂ ∧ PreRoot₁ = PreRoot₂ ∧ PostRoot₁ = PostRoot₂ ∧ IdComms₁ = IdComms₂ :=
+  Insertion_InputHash_injective reducedKeccak1568_collision_resistant
+
+end Insertion
+
+def main (_ : List String): IO UInt32 := pure 0
